\documentclass{article}
\usepackage{amssymb}
\usepackage{amsmath}

\begin{document}

Let $E_r$ be the $r \times r$ matrix whose all entries are 1's, 
and $I_r$ be the $r \times r$ identity matrix. 
Compute $({E_r - I_r \over r - 1})^n$ when $n \to \infty$.

\begin{align*}
({E_r - I_r \over r - 1})^n 
&= {1 \over (r - 1)^n} \sum_{k=0}^n {n \choose k} E_r^{n - k} I_n^k (-1)^k
\end{align*}

Notice that $E_r^k = r^{k - 1} E_r$ when $k > 0$
and $E_r^0 = I_n$.

Therefore

\begin{align*}
{1 \over (r - 1)^n} \sum_{k=0}^n {n \choose k} E_r^{n - k} I_r^k (-1)^k
&= {1 \over (r - 1)^n} 
	\left(I_r^n(-1)^n 
		+ E_r \sum_{k=0}^{n - 1} {n \choose k} r^{n - k - 1} (-1)^k
	\right) \\
&= {1 \over (r - 1)^n}
	\left((-1)^n I_n + {(r - 1)^n - (-1)^n \over r}E_r
	\right) \\
&= {(-1)^n \over (r - 1)^n} I_n + 
	\left({1 \over r} - {(-1)^n \over (r - 1)^n r}
	\right) E_r
\end{align*}

When $n \to \infty$, 
\begin{align*}
{(-1)^n \over (r - 1)^n} I_n + 
	\left({1 \over r} - {(-1)^n \over (r - 1)^n r}
	\right) E_r
&= {1 \over r} E_r
\end{align*}
\end{document}